Prove semantic preservation from `chor` to `pchor`

projection/proofs/bakery_to_halfProofScript.sml
@@ -1,347 +1,507 @@
-open preamble bakery_to_halfTheory congProofTheory semBakeryTheory semHalfBakeryTheory
+open preamble bakery_to_halfTheory congProofTheory
+open astBakeryTheory semBakeryTheory
+open astHalfBakeryTheory semHalfBakeryTheory
+open confluenceTheory
+
 
 val _ = new_theory "bakery_to_halfProof"
 
-val RTC_TRANS =  RTC_RULES |> CONV_RULE FORALL_AND_CONV
-                           |> CONJUNCTS |> el 2;
+Triviality RTC_TRANS =
+  RTC_RULES |> CONV_RULE FORALL_AND_CONV |> CONJUNCTS |> el 2
 
+Definition ptag_def:
+  ptag (semBakery$LTau p n)      = (semHalfBakery$LTau p n)
+∧ ptag (semBakery$LCom p v q x)  = (semHalfBakery$LCom p v q x)
+∧ ptag (semBakery$LSel p b q)    = (semHalfBakery$LSel p b q)
+∧ ptag (semBakery$LLet v p f vl) = (semHalfBakery$LLet v p f vl)
+End
 
-
-
-val trans_cTrm_def = Define `
-  
-`
-chorTrm_def
-
-Theorem trans_async_complete:
-  ∀s c α l ls s' c'.
-   trans (s,c) (α,l::ls) (s',c')
-   ⇒ trans (s',c') (l,ls) (state_from_tag s' l, chorTrm s' l c')
+Theorem freeprocs_p_eq:
+  ∀τ. freeprocs τ = freeprocs (ptag τ)
 Proof
-  `∀s c α τ s' c'. trans (s,c) (α,τ) (s',c')
-    ⇒ ∀l ls. τ = l::ls
-       ⇒ trans (s',c') (l,ls) (state_from_tag s' l, chorTrm s' l c')`
+  Cases
+  \\ fs [semHalfBakeryTheory.freeprocs_def,
+         semBakeryTheory.freeprocs_def,
+         ptag_def]
+QED
+
+Theorem project_inj:
+  ∀p q. project p = project q ⇒ p = q
+Proof
+  Induct \\ rw [project_def]
+  \\ Cases_on ‘q’ \\ fs [project_def]
+QED
+
+Theorem sync_trans_ptrans:
+  ∀s c τ s' c'.
+   trans (s,c) (τ,[]) (s',c')
+   ⇒ ptrans (s,project c) (ptag τ) (s',project c')
+Proof
+  ‘∀s c τ l s' c'.
+   trans (s,c) (τ,l) (s',c')
+   ⇒ l = []
+     ⇒ ptrans (s,project c) (ptag τ) (s',project c')’
   suffices_by metis_tac []
-  \\ ho_match_mp_tac semBakeryTheory.trans_pairind
+  \\ ho_match_mp_tac trans_pairind
+  \\ rw [project_def,
+         ptag_def,
+         ptrans_rules,
+         freeprocs_p_eq]
+  \\ fs [lcong_nil_simp,freeprocs_p_eq,ptrans_rules]
+QED
+
+Theorem ptrans_sync_trans:
+  ∀s c τ s' c'.
+   ptrans (s,project c) (ptag τ) (s',project c')
+   ⇒ trans (s,c) (τ,[]) (s',c')
+Proof
+  ‘∀s p γ s' q.
+   ptrans (s,p) γ (s',q)
+   ⇒ ∀c τ c'. γ = (ptag τ) ∧ p = (project c) ∧ q = (project c')
+     ⇒ trans (s,c) (τ,[]) (s',c')’
+  suffices_by metis_tac []
+  \\ ho_match_mp_tac ptrans_pairind
+  \\ rw [project_def,
+         ptag_def,
+         trans_rules,
+         freeprocs_p_eq]
+  \\ fs [lcong_nil_simp,freeprocs_p_eq,trans_rules]
+  (* First 9 goals *)
+  \\ TRY (Cases_on ‘τ’ \\ fs [ptag_def] \\ rveq
+          \\ Cases_on ‘c’ \\ fs [project_def]
+          \\ drule_then assume_tac project_inj
+          \\ rveq \\ fs [trans_rules] \\ NO_TAC)
+  (* Swap cases *)
+  \\ Cases_on ‘c’
+  \\ Cases_on ‘c'’
+  \\ fs [project_def] \\ rveq
+  \\ (irule trans_if_swap  ORELSE
+      irule trans_com_swap ORELSE
+      irule trans_sel_swap ORELSE
+      irule trans_let_swap)
+  \\ fs [freeprocs_p_eq]
+  \\ qexists_tac ‘[]’ \\ fs [lcong_sym]
+QED
+
+Theorem trans_sync_eq_ptrans_s:
+  ∀s c s' c'.
+   trans_sync (s,c) (s',c') ⇒ ptrans_s (s,project c) (s',project c')
+Proof
+  ‘∀p q. trans_sync p q
+    ⇒ ∀s c s' c'. p = (s,c) ∧ q = (s',c')
+       ⇒ ptrans_s (s,project c) (s',project c')’
+  suffices_by metis_tac []
+  \\ simp [trans_sync_def]
+  \\ ho_match_mp_tac RTC_ind
+  \\ rw [ptrans_s_def] \\ rw []
+  \\ Cases_on ‘p'’ \\ fs []
+  \\ drule_then assume_tac sync_trans_ptrans
+  \\ fs [ptrans_s_def]
+  \\ irule RTC_TRANS
+  \\ metis_tac []
+QED
+
+Definition lSyncTrm_def:
+  lSyncTrm (s,Nil) l = (s,Nil)
+∧ lSyncTrm (s,IfThen v p c1 c2) l = (if FLOOKUP s (v,p) = NONE
+                                     then (s,IfThen v p c1 c2)
+                                     else if (LTau p v) ⋲ l
+                                          then lSyncTrm (syncTrm (s,IfThen v p c1 c2) (LTau p v))
+                                                        (l − {|LTau p v|})
+                                          else if l = EMPTY_BAG then (s,IfThen v p c1 c2)
+                                               else lSyncTrm (chor_tl s (IfThen v p c1 c2)) l)
+∧ lSyncTrm (s,c) l   = (if (chor_tag c) ⋲ l
+                        then lSyncTrm (syncTrm (s,c) (chor_tag c)) (l − {|chor_tag c|})
+                        else if  l = EMPTY_BAG then (s,c)
+                             else lSyncTrm (chor_tl s c) l)
+Termination
+  WF_REL_TAC ‘measure (chor_size o SND o FST)’ \\ rw [chor_tag_def,chor_tl_def]
+  \\ rfs [chor_size_def,syncTrm_def,chor_match_def,chor_tl_def]
+  >- (Cases_on ‘FLOOKUP s (v,p)’ \\ fs [])
+  \\ every_case_tac \\ rw []
+  \\ Cases_on ‘FLOOKUP s (v,p)’ \\ fs []
+End
+
+(* Alternative induction principle *)
+Theorem lSyncTrm_pairind =
+  lSyncTrm_ind
+  |> Q.SPEC ‘λ(s,c) τ. P s c τ’
+  |> SIMP_RULE std_ss []
+  |> Q.GEN ‘P’
+
+Theorem trans_lSyncTrm:
+  ∀s c l.
+   no_self_comunication c ∧ no_undefined_vars (s,c)
+   ⇒ trans_sync (s,c) (lSyncTrm (s,c) l)
+Proof
+  ho_match_mp_tac lSyncTrm_pairind
+  \\ rw [lSyncTrm_def,trans_sync_refl,syncTrm_def,chor_tag_def,lrm_def,chor_match_def]
+  \\ fs [chor_tl_def]
+  \\ TRY (drule_then assume_tac no_undefined_FLOOKUP_if)
+  \\ TRY (drule_then assume_tac no_undefined_FLOOKUP_let)
+  \\ TRY (drule_then assume_tac no_undefined_FLOOKUP_com)
+  \\ fs [no_undefined_vars_def,
+         no_self_comunication_def,
+         free_variables_def,
+         DELETE_SUBSET_INSERT]
+  \\ rfs []
+  \\ rw [] \\ fs []
+  \\ irule trans_sync_step
+  \\ metis_tac [trans_rules]
+QED
+
+Theorem lcong_PERM:
+  ∀l l'. l τ≅ l' ⇒ PERM l l'
+Proof
+  ho_match_mp_tac lcong_ind
+  \\ rw [PERM_SYM]
+  >- metis_tac [PERM_TRANS]
+  \\ rw [PERM_APPEND_IFF]
+  \\ Cases_on ‘t1 = t2’ \\ fs []
+  \\ EVAL_TAC \\ rw []
+QED
+
+Theorem lSyncTrm_simps:
+  ∀p. lSyncTrm p {||} = p
+Proof
+  Cases \\ Cases_on ‘r’ \\ rw [lSyncTrm_def]
+QED
+
+Theorem lcong_LIST_TO_BAG:
+  ∀l l'. l τ≅ l' ⇒ LIST_TO_BAG l = LIST_TO_BAG l'
+Proof
+  rw [] \\ drule_then assume_tac lcong_PERM
+  \\ fs [GSYM PERM_LIST_TO_BAG]
+QED
+
+Theorem lcong_lSyncTrm:
+  ∀l l'. l τ≅ l' ⇒ ∀s c. lSyncTrm (s,c) (LIST_TO_BAG l) = lSyncTrm (s,c) (LIST_TO_BAG l')
+Proof
+  rw [] \\ drule_then assume_tac lcong_PERM
+  \\ fs [GSYM PERM_LIST_TO_BAG]
+QED
+
+(* Async trances can not contain LTau *)
+Theorem trans_l_not_tau:
+  ∀p τ l q. trans p (τ,l) q ⇒ ∀p v. ¬MEM (LTau p v) l
+Proof
+  rpt (gen_tac)
+  \\ Cases_on ‘p’
+  \\ Cases_on ‘q’
+  \\ MAP_EVERY Q.SPEC_TAC
+      (rev [(‘q'’,‘s’),(‘r’,‘c’),(‘τ’,‘τ’),(‘l’,‘l’),(‘q''’,‘s'’),(‘r'’,‘c'’)])
+  \\ ho_match_mp_tac trans_pairind
   \\ rw []
-
 QED
 
-
-
-
-val pchorTrm_def = Define`
-  pchorTrm s (semBakery$LCom p v q x) (Com p' v' q' x' c) =
-    (if (p,v,q,x) = (p',v',q',x') then project c
-     else if (p,v) = (p',v')
-     then PCom q x (p, THE (FLOOKUP s (v,p))) (pchorTrm s (LCom p v q x) c)
-     else Com p' v' q' x'     (pchorTrm s (LCom p v q x) c))
-∧ pchorTrm s (LSel p b q) (Sel p' b' q' c) =
-    (if (p,b,q) = (p',b',q') then project c
-     else if (p,b) = (p',b')
-     then PSel q (p, b) (pchorTrm s (LSel p b q) c)
-     else Sel p' b' q'  (pchorTrm s (LSel p b q) c))
-∧ pchorTrm s (LLet v p f vl) (Let v' p' f' vl' c) =
-    (if (v,p,f,vl) = (v',p',f',vl') then project c
-     else Let v' p' f' vl' (pchorTrm s (LLet v p f vl) c))
-∧ pchorTrm s (LTau p v) (IfThen v' p' c1 c2) =
-    (if (p,v) = (p',v')
-     then if FLOOKUP s (v,p) = SOME [1w] then project c1
-          else if ∃w. FLOOKUP s (v,p) = SOME w ∧ w ≠ [1w] then project c2
-          else IfThen v' p' (project c1) (project c2) (* Imposible? *)
-     else IfThen v' p' (pchorTrm s (LTau p v) c1) (pchorTrm s (LTau p v) c2))
-∧ pchorTrm s τ (Com p' v' q' x' c)  = Com p' v' q' x' (pchorTrm s τ c)
-∧ pchorTrm s τ (Sel p' b' q' c)     = Sel p' b' q' (pchorTrm s τ c)
-∧ pchorTrm s τ (Let v' p' f' vl' c) = Let v' p' f' vl' (pchorTrm s τ c)
-∧ pchorTrm s τ (IfThen v' p' c1 c2) = IfThen v' p' (pchorTrm s τ c1) (pchorTrm s τ c2)
-∧ pchorTrm s τ Nil                  = Nil
-`;
-
-val complete_pchor_def = Define `
-  complete_pchor Nil                = astBakery$Nil
-∧ complete_pchor (PCom q x (p,d) c) = complete_pchor c
-∧ complete_pchor (PSel q (p,b) c)   = complete_pchor c
-∧ complete_pchor (Com p v q x c)    = Com p v q x (complete_pchor c)
-∧ complete_pchor (Sel p b q c)      = Sel p b q   (complete_pchor c)
-∧ complete_pchor (Let v p f vl c)   = Let v p f vl (complete_pchor c)
-∧ complete_pchor (IfThen v p c1 c2) = IfThen v p (complete_pchor c1) (complete_pchor c2)
-`
-
-Theorem complete_project_eq:
-  ∀c. complete_pchor (project c) = c
+(* Async trances can not contain LLet *)
+Theorem trans_l_not_let:
+  ∀p τ l q. trans p (τ,l) q ⇒ ∀v p f vl. ¬MEM (LLet v p f vl) l
 Proof
-  Induct \\ rw [complete_pchor_def,project_def]
+  rpt (gen_tac)
+  \\ Cases_on ‘p’
+  \\ Cases_on ‘q’
+  \\ MAP_EVERY Q.SPEC_TAC
+      (rev [(‘q'’,‘s’),(‘r’,‘c’),(‘τ’,‘τ’),(‘l’,‘l’),(‘q''’,‘s'’),(‘r'’,‘c'’)])
+  \\ ho_match_mp_tac trans_pairind
+  \\ rw []
 QED
-
-Theorem no_undefined_vars_from_tags:
-  ∀c s α.
-   no_undefined_vars (s,c) ⇒ no_undefined_vars (state_from_tag s α, c)
+(* Tags in the async trace need to be part of the original tag freeprocs (COM) *)
+Theorem trans_l_freeprocs_com:
+  ∀p τ l q.
+   trans p (τ,l) q
+   ⇒ ∀c1 v1 c2 v2.
+      MEM (LCom c1 v1 c2 v2) l
+      ⇒ c1 ∈ freeprocs τ ∨ c2 ∈ freeprocs τ
 Proof
-  rw [no_undefined_vars_def,free_variables_def]
-  \\ Cases_on `α` \\ fs [state_from_tag_def]
-  \\ ho_match_mp_tac SUBSET_TRANS
-  \\ metis_tac [SUBSET_OF_INSERT]
+  rpt (gen_tac)
+  \\ Cases_on ‘p’
+  \\ Cases_on ‘q’
+  \\ MAP_EVERY Q.SPEC_TAC
+      (rev [(‘q'’,‘s’),(‘r’,‘c’),(‘τ’,‘τ’),(‘l’,‘l’),(‘q''’,‘s'’),(‘r'’,‘c'’)])
+  \\ ho_match_mp_tac trans_pairind
+  \\ rw []
+  \\ metis_tac []
 QED
 
-Theorem chorTrm_eq_pchorTrm:
-  ∀c s α. chorTrm s α c = complete_pchor (pchorTrm s α c)
-
-
-Theorem Trm_trans:
-  ∀c s α. no_undefined_vars (state_from_tag s α,c) ∧ no_self_comunication c
-   ⇒ ∃s'. trans_s (state_from_tag s α, chorTrm s α c) (s', complete_pchor (pchorTrm s α c))
+(* Tags in the async trace need to be part of the original tag freeprocs (SEL) *)
+Theorem trans_l_freeprocs_sel:
+  ∀p τ l q.
+   trans p (τ,l) q
+   ⇒ ∀c1 b c2.
+      MEM (LSel c1 b c2) l
+      ⇒ c1 ∈ freeprocs τ ∨ c2 ∈ freeprocs τ
 Proof
-  ho_match_mp_tac (theorem "pchorTrm_ind")
-  \\ rw [chorTrm_def,pchorTrm_def,complete_pchor_def,complete_project_eq]
-  \\ TRY (qmatch_goalsub_abbrev_tac `trans_s (s1,c1) (_,c1)`
-         \\ qexists_tac `s1`
-         \\ rw [semBakeryTheory.trans_s_def])
-  >- (qmatch_asmsub_abbrev_tac `no_undefined_vars (s1,c)`
-     \\ `no_undefined_vars (s1,c)`
-        by (UNABBREV_ALL_TAC \\ fs [ no_undefined_vars_def,state_from_tag_def
-                                   , free_variables_def,no_self_comunication_def]
-
-
-  Induct
-  \\ rw [chorTrm_def,pchorTrm_def,complete_pchor_def,complete_project_eq]
-  >- (qexists_tac `state_from_tag s α` \\ rw [semBakeryTheory.trans_s_def])
-  >- (`no_undefined_vars (state_from_tag s' α,c)  ∧
-       no_undefined_vars (state_from_tag s' α,c') ∧
-       no_self_comunication c    ∧
-       no_self_comunication c'`
-       by fs [ no_undefined_vars_def,free_variables_def
-             , no_self_comunication_def,no_undefined_vars_from_tags]
-     \\ first_x_assum drule \\ disch_then drule
-     \\ first_x_assum drule \\ disch_then drule
-     \\ rw []
-     \\ Cases_on `∃p v. α = LTau v p` \\ rw []
-     >- (Cases_on `(v,p) = (l,s)`
-        \\ rw [chorTrm_def,pchorTrm_def,complete_pchor_def,pchorTrm_def,complete_project_eq]
-        \\ TRY (qmatch_goalsub_abbrev_tac `trans_s (s1,c1) (_,c1)`
-        \\ qexists_tac `s1`
-        \\ rw [semBakeryTheory.trans_s_def])
-
-
-
-complete_pchor_def
-
-
-
-
-first_x_assum (drule_then ) rw []
-
-rw []
-     \\ cheat)
-  \\ cheat
+  rpt (gen_tac)
+  \\ Cases_on ‘p’
+  \\ Cases_on ‘q’
+  \\ MAP_EVERY Q.SPEC_TAC
+      (rev [(‘q'’,‘s’),(‘r’,‘c’),(‘τ’,‘τ’),(‘l’,‘l’),(‘q''’,‘s'’),(‘r'’,‘c'’)])
+  \\ ho_match_mp_tac trans_pairind
+  \\ rw []
+  \\ metis_tac []
 QED
 
-
-Theorem Trm_preservation:
-  ∀c s α τ.
-   trans (s,c) (α,τ) (state_from_tag s α, chorTrm s α c) ∧
+Theorem trans_lSyncTrm_chorTrm:
+  ∀c s τ l s' c'.
+   no_self_comunication c  ∧
    no_undefined_vars (s,c) ∧
-   no_self_comunication c
-   ⇒ ∃s'. trans_s (state_from_tag s α, chorTrm s α c)
-                  (s',complete_pchor (pchorTrm s α c)) ∧
-          trans_s (s,project c)
-                  (s',project (complete_pchor (pchorTrm s α c)))
+   trans (s,c) (τ,l) (s',c')
+   ⇒ trans_sync (s,c) (lSyncTrm (s',c') (LIST_TO_BAG l))
 Proof
-  `∀s c α τ s1 c1.
-    trans (s,c) (α,τ) (s1,c1)
-    ⇒ (no_undefined_vars (s,c) ∧
-       no_self_comunication c  ∧
-       s1 = state_from_tag s α ∧
-       c1 = chorTrm s α c
-       ⇒ ∃s'. trans_s (state_from_tag s α, chorTrm s α c)
-                      (s',complete_pchor (pchorTrm s α c)) ∧
-              trans_s (s,project c)
-                      (s',project (complete_pchor (pchorTrm s α c))))`
-         suffices_by metis_tac []
-  \\ ho_match_mp_tac semBakeryTheory.trans_pairind
-  \\ rw [chorTrm_def,pchorTrm_def,complete_pchor_def]
-
-
-
-
-Theorem preservation:
-  ∀c s α τ s' c'.
-   trans (s,c) (α,τ) (s',c') ∧
-   no_undefined_vars (s,c) ∧
-   no_self_comunication c
-   ⇒ ∃c'' s''. trans_s (s',c') (s'',c'')
-      ∧        trans_s (s,project c) (s'',project c'')
-Proof
-  `∀s c α τ s' c'.
-   trans (s,c) (α,τ) (s',c')
-   ⇒  no_undefined_vars (s,c) ∧
-      no_self_comunication c
-      ⇒ ∃c'' s''. trans_s (s',c') (s'',c'')
-         ∧        trans_s (s,project c) (s'',project c'')`
-  suffices_by metis_tac []
-  \\ let
-    val one2one = qmatch_goalsub_abbrev_tac `semBakery$trans_s (st,chor) _`
-                  \\ map_every qexists_tac [`chor`,`st`]
-                  \\ unabbrev_all_tac
-                  \\ rw [trans_s_def,semBakeryTheory.trans_s_def]
-                  \\ ho_match_mp_tac RTC_SINGLE
-                  \\ metis_tac [trans_rules,project_def]
-  in ho_match_mp_tac semBakeryTheory.trans_pairind \\ rw []
-     >- one2one >- one2one >- one2one >- one2one >- one2one
-  end
-    (* IfThen swap *)
-  >- (`no_undefined_vars (s,c)  ∧
-          no_undefined_vars (s,c') ∧
-          no_self_comunication c    ∧
-          no_self_comunication c'`
-          by fs [ no_undefined_vars_def,free_variables_def
-                , no_self_comunication_def]
-      \\ first_x_assum drule \\ disch_then drule
-      \\ first_x_assum drule \\ disch_then drule
-      \\ rw []
-      \\ `∃d. FLOOKUP s' (v,p) = SOME d ∧ FLOOKUP s (v,p) = SOME d`
-          by (drule trans_state
-              \\ rw [] \\ fs []
-              \\ Cases_on `α`
-              \\ fs [ state_from_tag_def
-                    , semBakeryTheory.freeprocs_def
-                    , no_undefined_vars_def
-                    , free_variables_def,FLOOKUP_DEF]
-              \\ EVAL_TAC
-              \\ fs [])
-      \\ Cases_on `d = [1w]`
-      >- (map_every qexists_tac [`c''''`,`s''`]
-         \\ conj_tac
-         >- (fs [semBakeryTheory.trans_s_def]
-            \\ ho_match_mp_tac RTC_TRANS
-            \\ metis_tac [semBakeryTheory.trans_rules])
-         \\ rw [project_def]
-         \\ fs [trans_s_def]
-         \\ ho_match_mp_tac RTC_TRANS
-         \\ metis_tac [trans_rules])
-      >- (map_every qexists_tac [`c'''''`,`s'''`]
-         \\ conj_tac
-         >- (fs [semBakeryTheory.trans_s_def]
-            \\ ho_match_mp_tac RTC_TRANS
-            \\ metis_tac [semBakeryTheory.trans_rules])
-         \\ rw [project_def]
-         \\ fs [trans_s_def]
-         \\ ho_match_mp_tac RTC_TRANS
-         \\ metis_tac [trans_rules]))
-
-  >- (`trans (s,IfThen v p c c') (α,τ) (s',IfThen v p c'' c''')`
-      by metis_tac [semBakeryTheory.trans_if_swap]
-      \\ drule trans_imp_chorTrm
-      \\ drule trans_state \\ rw []
-      \\ drule Trm_trans
-      \\ disch_then (qspec_then `α` drule)
-      \\ rw [] \\ asm_exists_tac  \\ rw []
-      \\
-
-
-)
-
-
-
-
-
-
   Induct
-  >- cheat (* trans_nil_false *)
-  >- (rw [] \\ pop_assum (assume_tac o PURE_ONCE_REWRITE_RULE [semBakeryTheory.trans_cases])
+  >- fs [Once trans_cases]
+  \\ rw []
+  \\  qpat_x_assum `trans _ _ _`
+                   (ASSUME_TAC o SIMP_RULE std_ss [Once trans_cases])
+  \\ rw [] >> rfs [] >> rw []
+  (* If-Normal *)
+  >- (irule trans_sync_step
+      \\ MAP_EVERY qexists_tac [‘(s',c)’,‘LTau l s’]
+      \\ reverse conj_tac
+      >- metis_tac [trans_rules]
+      \\ Cases_on ‘c’ \\ fs [lSyncTrm_def,trans_sync_refl])
+  (* If-Swap-Sync*)
+  >- (irule trans_sync_step
+      \\ MAP_EVERY qexists_tac [‘(s',c')’,‘LTau l s’]
+      \\ reverse conj_tac
+      >- metis_tac [trans_rules]
+      \\ Cases_on ‘c'’ \\ fs [lSyncTrm_def,trans_sync_refl])
+  (*  If-Swap-Async*)
+  >- (rw []
+      \\ qpat_assum ‘trans _ _ (s'',_)’ mp_tac
+      \\ disch_then (mp_then Any assume_tac trans_state) \\ rveq
+      \\ drule_then assume_tac no_undefined_FLOOKUP_if \\ fs []
+      \\ rw [lSyncTrm_def]
+      >- (Cases_on ‘τ’
+          \\ fs [state_from_tag_def,
+                 semBakeryTheory.freeprocs_def,
+                 FLOOKUP_UPDATE] \\ rfs [])
+      >- metis_tac [IN_LIST_TO_BAG,trans_l_not_tau]
+      >- (rfs [LIST_TO_BAG_EQ_EMPTY] \\ rveq
+          \\ fs [lcong_nil_simp]
+          \\ irule trans_sync_one \\ qexists_tac ‘τ’
+          \\ irule trans_if_swap  \\ fs []
+          \\ qexists_tac ‘[]’ \\ fs [lcong_sym])
+      \\ Cases_on ‘x = [1w]’ \\ fs []
+      \\ ho_match_mp_tac trans_sync_step
+      (* True branch *)
+      >- (drule_then (qspecl_then [‘c’,‘c'’] assume_tac) trans_if_true
+          \\ asm_exists_tac \\ fs []
+          \\ qmatch_goalsub_abbrev_tac ‘chor_tl sτ’
+          \\ ‘FLOOKUP sτ (s,l) = SOME [1w]’
+              by (UNABBREV_ALL_TAC
+                  \\ Cases_on ‘τ’
+                  \\ fs [state_from_tag_def,
+                         semBakeryTheory.freeprocs_def,
+                         FLOOKUP_UPDATE]
+                  \\ rfs [])
+          \\ rw [lSyncTrm_def,chor_tl_def]
+          \\ first_x_assum irule
+          \\ fs [no_self_comunication_def,
+                 no_undefined_vars_def,
+                 free_variables_def]
+          \\ asm_exists_tac \\ fs [])
+      (* False branch *)
+      \\ drule_then (qspecl_then [‘c’,‘c'’] assume_tac) trans_if_false \\ rfs []
+      \\ asm_exists_tac \\ fs []
+      \\ qmatch_goalsub_abbrev_tac ‘chor_tl sτ’
+      \\ ‘FLOOKUP sτ (s,l) = SOME x ∧ x ≠ [1w]’
+          by (UNABBREV_ALL_TAC
+              \\ Cases_on ‘τ’
+              \\ fs [state_from_tag_def,
+                     semBakeryTheory.freeprocs_def,
+                     FLOOKUP_UPDATE]
+              \\ rfs [])
+      \\ rw [lSyncTrm_def,chor_tl_def]
+      \\ drule_then assume_tac lcong_LIST_TO_BAG \\ fs []
+      \\ first_x_assum irule
+      \\ fs [no_self_comunication_def,
+             no_undefined_vars_def,
+             free_variables_def]
+      \\ asm_exists_tac \\ fs [])
+  (* Com-Normal *)
+  >- (irule trans_sync_step
+      \\ qmatch_goalsub_abbrev_tac ‘lSyncTrm (s'',_)’
+      \\ MAP_EVERY qexists_tac [‘(s'',c)’,‘LCom l0 s0 l s’]
+      \\ reverse conj_tac
+      >- metis_tac [trans_rules,trans_sync_refl]
+      \\ Cases_on ‘c’ \\ fs [lSyncTrm_def,trans_sync_refl])
+  (* Com-Swap *)
+  >- (drule_then assume_tac trans_state \\ rveq
+      \\ drule_then assume_tac no_undefined_FLOOKUP_com \\ fs []
+      \\ rw [lSyncTrm_def]
+      >- (fs [IN_LIST_TO_BAG,chor_tag_def]
+          \\ drule_then drule trans_l_freeprocs_com
+          \\ fs [])
+      >- (rfs [LIST_TO_BAG_EQ_EMPTY] \\ rveq
+          \\ irule trans_sync_one \\ qexists_tac ‘τ’
+          \\ irule trans_com_swap  \\ fs [])
+      \\ qmatch_goalsub_abbrev_tac ‘chor_tl sτ’
+      \\ ‘FLOOKUP sτ (s0,l0) = SOME x’
+          by (UNABBREV_ALL_TAC
+              \\ Cases_on ‘τ’
+              \\ fs [state_from_tag_def,
+                     semBakeryTheory.freeprocs_def,
+                     FLOOKUP_UPDATE]
+              \\ rfs [])
+      \\ rw [chor_tl_def,FLOOKUP_UPDATE]
+      \\ ho_match_mp_tac trans_sync_step
+      \\ fs [no_self_comunication_def]
+      \\ qspec_then ‘s'’ mp_tac trans_com
+      \\ disch_then drule
+      \\ disch_then (drule_then (qspecl_then [‘s’,‘c’] assume_tac))
+      \\ asm_exists_tac \\ fs []
+      \\ first_x_assum irule
+      \\ fs [no_undefined_vars_def,
+             free_variables_def,
+             DELETE_SUBSET_INSERT]
+      \\ qexists_tac ‘τ’
+      \\ irule semantics_add_irrelevant_state \\ fs [])
+  (* Com-Async *)
+  >- (rw [lSyncTrm_def,chor_tag_def,syncTrm_def,chor_match_def,chor_tl_def]
+      \\ drule_then assume_tac trans_state \\ rveq
+      \\ drule_then assume_tac no_undefined_FLOOKUP_com \\ fs [no_self_comunication_def]
+      \\ qmatch_goalsub_abbrev_tac ‘FLOOKUP sτ’
+      \\ drule_then drule trans_com
+      \\ disch_then (qspecl_then [‘s’,‘c’] assume_tac)
+      \\ ‘FLOOKUP sτ (s0,l0) = SOME x’
+              by (UNABBREV_ALL_TAC
+                  \\ Cases_on ‘τ’
+                  \\ fs [state_from_tag_def,
+                         semBakeryTheory.freeprocs_def,
+                         semBakeryTheory.written_def,
+                         FLOOKUP_UPDATE]
+                  \\ rfs [])
+      \\ ho_match_mp_tac trans_sync_step
+      \\ asm_exists_tac \\ fs []
+      \\ first_x_assum irule
+      \\ fs [no_undefined_vars_def,
+             free_variables_def,
+             DELETE_SUBSET_INSERT]
+      \\ qexists_tac ‘τ’
+      \\ irule semantics_add_irrelevant_state2 \\ fs []
+      \\ Cases_on ‘τ’
+      \\ fs [semBakeryTheory.written_def,
+             semBakeryTheory.read_def,
+             semBakeryTheory.freeprocs_def] \\ rfs []
+      \\ qpat_x_assum ‘l ≠ l'’ mp_tac
+      \\ rpt (last_x_assum (K ALL_TAC))
+      \\ Induct_on ‘l0'’ \\ fs [])
+  (* Let-Normal *)
+  >- (irule trans_sync_step
+      \\ qmatch_goalsub_abbrev_tac ‘lSyncTrm (s'',_)’
+      \\ MAP_EVERY qexists_tac [‘(s'',c)’,‘LLet s l0 f l’]
+      \\ reverse conj_tac
+      >- metis_tac [trans_rules,trans_sync_refl]
+      \\ Cases_on ‘c’ \\ fs [lSyncTrm_def,trans_sync_refl])
+  (* Let-Swap *)
+  >- (drule_then assume_tac trans_state \\ rveq
+     \\ drule_then assume_tac no_undefined_FLOOKUP_let \\ fs []
+     \\ rw [lSyncTrm_def]
+     >- (fs [IN_LIST_TO_BAG,chor_tag_def]
+         \\ metis_tac [trans_l_not_let])
+     >- (rfs [LIST_TO_BAG_EQ_EMPTY] \\ rveq
+         \\ irule trans_sync_one \\ qexists_tac ‘τ’
+         \\ irule trans_let_swap  \\ fs [])
+     \\ qmatch_goalsub_abbrev_tac ‘chor_tl sτ’
+     \\ rw [chor_tl_def,FLOOKUP_UPDATE]
+     \\ ho_match_mp_tac trans_sync_step
+     \\ fs [no_self_comunication_def]
+     \\ qspec_then ‘s'’ mp_tac trans_let
+     \\ disch_then drule
+     \\ disch_then (qspecl_then [‘s’,‘f’,‘c’] assume_tac)
+     \\ asm_exists_tac \\ fs []
+     \\ first_x_assum irule
+     \\ fs [no_undefined_vars_def,
+            free_variables_def,
+            DELETE_SUBSET_INSERT]
+     \\ qexists_tac ‘τ’
+     \\ qmatch_goalsub_abbrev_tac ‘f s0’
+     \\ qmatch_goalsub_abbrev_tac ‘(sτ |+ (_, f s1))’
+     \\ ‘s0 = s1’ by
+         (UNABBREV_ALL_TAC
+          \\ Cases_on ‘τ’
+          \\ fs [state_from_tag_def,
+                 semBakeryTheory.freeprocs_def,
+                 FLOOKUP_UPDATE]
+          \\ rfs []
+          \\ qpat_x_assum ‘l0 ≠ _'’ mp_tac
+          \\ rpt (last_x_assum (K ALL_TAC))
+          \\ Induct_on ‘l’ \\ rw [] \\ fs [FLOOKUP_UPDATE])
+     \\ fs [] \\ irule semantics_add_irrelevant_state2
      \\ fs []
-     >- (map_every qexists_tac [`c`,`s'`]
-        \\ rw [semBakeryTheory.trans_s_def,trans_s_def,project_def]
-        \\ ho_match_mp_tac RTC_SINGLE
-        \\ metis_tac [trans_rules])
-     >- (map_every qexists_tac [`c'`,`s'`]
-        \\ rw [semBakeryTheory.trans_s_def,trans_s_def,project_def]
-        \\ ho_match_mp_tac RTC_SINGLE
-        \\ metis_tac [trans_rules])
-     >- (first_x_assum drule
-        \\ first_x_assum drule
-        \\ rw []
-       )
-
-
-  >- (`no_undefined_vars (s,c)`
-      by (drule trans_state
-         \\ rw [] \\ fs []
-         \\ fs []
-  )
-
-trans_if_swap
-
-
+     \\ Cases_on ‘τ’
+     \\ fs [semBakeryTheory.written_def,
+            semBakeryTheory.read_def,
+            semBakeryTheory.freeprocs_def] \\ rfs []
+     \\ qpat_x_assum ‘l0 ≠ l''’ mp_tac
+     \\ rpt (last_x_assum (K ALL_TAC))
+     \\ Induct_on ‘l0'’ \\ fs [])
+  (* Sel-Normal *)
+  >- (irule trans_sync_step
+      \\ qmatch_goalsub_abbrev_tac ‘lSyncTrm (s'',_)’
+      \\ MAP_EVERY qexists_tac [‘(s'',c)’,‘LSel l0 b l’]
+      \\ reverse conj_tac
+      >- metis_tac [trans_rules,trans_sync_refl]
+      \\ Cases_on ‘c’ \\ fs [lSyncTrm_def,trans_sync_refl])
+  (* Let-Swap *)
+  >- (rw [lSyncTrm_def,chor_tag_def,syncTrm_def,chor_match_def,chor_tl_def]
+      >- (fs [IN_LIST_TO_BAG,chor_tag_def]
+          \\ drule_then drule trans_l_freeprocs_sel
+          \\ fs [])
+      >- (rfs [LIST_TO_BAG_EQ_EMPTY] \\ rveq
+          \\ irule trans_sync_one \\ qexists_tac ‘τ’
+          \\ irule trans_sel_swap  \\ fs [])
+      \\ ho_match_mp_tac trans_sync_step
+      \\ fs [no_self_comunication_def]
+      \\ qspec_then ‘s’ mp_tac trans_sel
+      \\ disch_then drule
+      \\ disch_then (qspecl_then [‘b’,‘c’] assume_tac)
+      \\ asm_exists_tac \\ fs []
+      \\ first_x_assum irule
+      \\ fs [no_undefined_vars_def,
+             free_variables_def,
+             DELETE_SUBSET_INSERT]
+      \\ asm_exists_tac \\ fs [])
+  (* Let-Async *)
+  \\ rw [lSyncTrm_def,chor_tag_def,syncTrm_def,chor_match_def,chor_tl_def]
+  \\ ho_match_mp_tac trans_sync_step
+  \\ fs [no_self_comunication_def]
+  \\ qspec_then ‘s’ mp_tac trans_sel
+  \\ disch_then drule
+  \\ disch_then (qspecl_then [‘b’,‘c’] assume_tac)
+  \\ asm_exists_tac \\ fs []
+  \\ first_x_assum irule
+  \\ fs [no_undefined_vars_def,
+         free_variables_def,
+         DELETE_SUBSET_INSERT]
+  \\ asm_exists_tac \\ fs []
+QED
 
 Theorem preservation:
   ∀s c α τ s' c'.
+   no_self_comunication c ∧
    no_undefined_vars (s,c) ∧
    trans (s,c) (α,τ) (s',c')
-   ⇒ ∃c'' s''. trans_s (s',c') (s'',c'')
-      ∧        trans_s (s,project c) (s'',project c'')
+   ⇒ ∃c'' s''.
+      trans_sync (s',c') (s'',c'') ∧
+      ptrans_s (s,project c) (s'',project c'')
 Proof
-  `∀s c α τ s' c' .
-   trans (s,c) (α,τ) (s',c')
-   ⇒ no_undefined_vars (s,c)
-     ⇒ ∃c'' s''. trans_s (s',c') (s'',c'')
-        ∧        trans_s (s,project c) (s'',project c'')`
-  suffices_by metis_tac [] >>
-  let
-    val one2one = qmatch_goalsub_abbrev_tac `semBakery$trans_s (st,chor) _`
-                  \\ map_every qexists_tac [`chor`,`st`]
-                  \\ unabbrev_all_tac
-                  \\ rw [trans_s_def,semBakeryTheory.trans_s_def]
-                  \\ ho_match_mp_tac RTC_SINGLE
-                  \\ metis_tac [trans_rules,project_def]
-  in ho_match_mp_tac semBakeryTheory.trans_pairind \\ rw []
-     >- one2one >- one2one >- one2one >- one2one >- one2one
-  end
-  (* IfThen swap *)
-  >- (`no_undefined_vars (s,c) ∧ no_undefined_vars (s,c')`
-      by fs [no_undefined_vars_def,free_variables_def]
-      \\ first_x_assum drule
-      \\ first_x_assum drule
-      \\ rw []
-      \\ `no_undefined_vars (s',c'') ∧ no_undefined_vars (s',c''')`
-         by (rw [] \\ ho_match_mp_tac no_undefined_vars_trans_pres
-            \\ metis_tac [])
-      \\ `∃d. FLOOKUP s' (v,p) = SOME d ∧ FLOOKUP s (v,p) = SOME d`
-         by (drule trans_state
-            \\ rw [] \\ fs []
-            \\ Cases_on `α`
-            \\ fs [ state_from_tag_def
-                  , semBakeryTheory.freeprocs_def
-                  , no_undefined_vars_def
-                  , free_variables_def,FLOOKUP_DEF]
-            \\ EVAL_TAC
-            \\ fs [])
-      \\ Cases_on `d = [1w]`
-      >- (map_every qexists_tac [`c''''`,`s''`]
-         \\ conj_tac
-         >- (fs [semBakeryTheory.trans_s_def]
-            \\ ho_match_mp_tac RTC_TRANS
-            \\ metis_tac [semBakeryTheory.trans_rules])
-         \\ rw [project_def]
-         \\ fs [trans_s_def]
-         \\ ho_match_mp_tac RTC_TRANS
-         \\ metis_tac [trans_rules])
-      >- (map_every qexists_tac [`c'''''`,`s'''`]
-         \\ conj_tac
-         >- (fs [semBakeryTheory.trans_s_def]
-            \\ ho_match_mp_tac RTC_TRANS
-            \\ metis_tac [semBakeryTheory.trans_rules])
-         \\ rw [project_def]
-         \\ fs [trans_s_def]
-         \\ ho_match_mp_tac RTC_TRANS
-         \\ metis_tac [trans_rules]))
-  >- (`no_undefined_vars (s,c)`
-      by (drule trans_state
-         \\ rw [] \\ fs []
-         \\ fs []
-  )
-
-
-
-semBakeryTheory.trans_if_true
-
+  rpt (strip_tac)
+  \\ drule_then drule no_undefined_vars_trans_pres
+  \\ drule_then drule no_self_comunication_trans_pres
+  \\ disch_then (mp_then Any assume_tac trans_lSyncTrm)
+  \\ first_x_assum (disch_then o (mp_then Any (qspec_then ‘LIST_TO_BAG τ’ assume_tac)))
+  \\ Cases_on ‘lSyncTrm (s',c') (LIST_TO_BAG τ)’
+  \\ asm_exists_tac
+  \\ fs []
+  \\ ho_match_mp_tac trans_sync_eq_ptrans_s
+  \\ first_x_assum (assume_tac o GSYM) \\ fs []
+  \\ first_x_assum (K ALL_TAC)
+  \\ ho_match_mp_tac trans_lSyncTrm_chorTrm
+  \\ asm_exists_tac \\ fs []
+  \\ asm_exists_tac \\ fs []
 QED
+
+val _ = export_theory ()
